Remove tuples from STLC and r1cs

R1cs.v
@@ -20,43 +20,42 @@ Module R1CS(PF: GaloisField).
   Import VectorNotations.
   Definition Vfp := Vector.t Fp.
   
-  Inductive term: nat -> nat -> nat -> Set :=
-  | input: forall (n: nat), term (S n) 0 0
-  | output: forall (n: nat), term 0 (S n) 0
-  | var: forall (n: nat), term 0 0 (S n)
-  | one: term 0 0 0.
+  Inductive term: nat -> nat -> Set :=
+  | input: forall (n: nat), term (S n) 0
+  | output: term 0 0
+  | var: forall (n: nat), term 0 (S n)
+  | one: term 0 0.
 
-  Inductive additions: nat -> nat -> nat -> Type :=
-  | ahead: forall i o v, Fp * term i o v -> additions i o v
-  | atail: forall i o v i' o' v',
-      Fp * term i o v ->
-      additions i' o' v' ->
-      additions (max i i') (max o o') (max v v').
+  Inductive additions: nat -> nat -> Type :=
+  | ahead: forall i v, Fp * term i v -> additions i v
+  | atail: forall i v i' v',
+      Fp * term i v ->
+      additions i' v' ->
+      additions (max i i') (max v v').
   
-  Inductive constraint: nat -> nat -> nat -> Type :=
-  | lc: forall i o v i' o' v' i'' o'' v''
-      (A: additions i o v)
-      (B: additions i' o' v')
-      (C: additions i'' o'' v''),
-      constraint (max i (max i' i'')) (max o (max o' o'')) (max v (max v' v'')).
+  Inductive constraint: nat -> nat -> Type :=
+  | lc: forall i v i' v' i'' v''
+      (A: additions i v)
+      (B: additions i' v')
+      (C: additions i'' v''),
+      constraint (max i (max i' i'')) (max v (max v' v'')).
 
-  Inductive r1cs: nat -> nat -> nat -> nat -> Type :=
-  | rnil: r1cs 0 0 0 0
-  | rcons: forall n i o v i' o' v',
-      constraint i o v ->
-      r1cs n i' o' v' ->
-      r1cs (S n) (max i i') (max o o') (max v v').
-
+  Inductive r1cs: nat -> nat -> nat -> Type :=
+  | rnil: r1cs 0 0 0
+  | rcons: forall n i v i' v',
+      constraint i v ->
+      r1cs n i' v' ->
+      r1cs (S n) (max i i') (max v v').
   
-  Arguments additions {i} {o} {v}.
-  Arguments ahead {i} {o} {v}.
-  Arguments atail {i} {o} {v} {i'} {o'} {v'}.
-  Arguments constraint {i} {o} {v}.
-  Arguments lc {i} {o} {v} {i'} {o'} {v'} {i''} {o''} {v''}.
-  Arguments rcons {n} {i} {o} {v} {i'} {o'} {v'}.
-  Arguments r1cs {n} {i} {o} {v}.
+  Arguments additions {i} {v}.
+  Arguments ahead {i} {v}.
+  Arguments atail {i} {v} {i'} {v'}.
+  Arguments constraint {i} {v}.
+  Arguments lc {i} {v} {i'} {v'} {i''} {v''}.
+  Arguments rcons {n} {i} {v} {i'} {v'}.
+  Arguments r1cs {n} {i} {v}.
   
-  Definition r1cs_singleton{i o v}(c: @constraint i o v) :=
+  Definition r1cs_singleton{i v}(c: @constraint i v) :=
     rcons c rnil.
 
   (** syntax *)
@@ -93,10 +92,9 @@ Module R1CS(PF: GaloisField).
           n constr,
           z constr).
   
-  Notation "z 'o[' n ']'" :=
-    (to_p z, output n%nat)
+  Notation "z 'o'" :=
+    (to_p z, output)
       (in custom r1cs at level 4,
-          n constr,
           z constr).
   
   Notation "z 'v[' n ']'" :=
@@ -111,45 +109,43 @@ Module R1CS(PF: GaloisField).
           z constr at level 0).
 
   Coercion r1cs_singleton: constraint >-> r1cs.
-  Eval cbn in <[ { (3o[0] + 3i[1]) * (3i[0] + 2v[2]) == ([1]) };{ (3o[0] + 3i[1]) * (3i[0] + 2v[2]) == ([1]) }  ]>.   
+  Eval cbn in <[
+                { (3o + 3i[1]) * (3i[0] + 2v[2]) == ([1]) };
+              { (3o + 3i[1]) * (3i[0] + 2v[2]) == ([1]) }  ]>.   
 
-  Fixpoint eval_additions{i o v i' o' v'}
-           (adds: @additions i o v)
+  Fixpoint eval_additions{i v i' v'}
+           (adds: @additions i v)
            (inputs: Vfp i')
-           (outputs: Vfp o')
-           (vars: Vfp v'): i <= i' -> o <= o' -> v <= v' -> Fp.
+           (output: Fp)
+           (vars: Vfp v'): i <= i' -> v <= v' -> Fp.
     invert adds; intros.
-    - invert H; invert H4.
-      + apply le_lt_Sn_m in H0; clear H1 H2.
-        exact (pkmul H3 (Vector.nth inputs (Fin.of_nat_lt H0))).  (** Fp * Input term *)
-      + apply le_lt_Sn_m in H1; clear H0 H2.
-        exact (pkmul H3 (Vector.nth outputs (Fin.of_nat_lt H1))). (** Fp * Output term *)
-      + apply le_lt_Sn_m in H2; clear H0 H1.
-        exact (pkmul H3 (Vector.nth vars (Fin.of_nat_lt H2))).    (** Fp * Var term *)
-      + exact H3. (** Fp * 1 (One) term *)
-    - specialize (eval_additions _ _ _ _ _ _ H0 inputs outputs vars) as Hprev.
+    - invert H; invert H3.
+      + apply le_lt_Sn_m in H0.
+        exact (pkmul H2 (Vector.nth inputs (Fin.of_nat_lt H0))).  (** Fp * Input term *)
+      + exact (pkmul H2 output). (** Fp * Output term *)
+      + apply le_lt_Sn_m in H1.
+        exact (pkmul H2 (Vector.nth vars (Fin.of_nat_lt H1))).    (** Fp * Var term *)
+      + exact H2. (** Fp * 1 (One) term *)
+    - specialize (eval_additions _ _ _ _ H0 inputs output vars) as Hprev.
       pose proof (Nat.max_lub_r _ _ _ H1).
       pose proof (Nat.max_lub_r _ _ _ H2).
-      pose proof (Nat.max_lub_r _ _ _ H3).
       pose proof (Nat.max_lub_l _ _ _ H1).
       pose proof (Nat.max_lub_l _ _ _ H2).
-      pose proof (Nat.max_lub_l _ _ _ H3).
-      clear H1 H2 H3.
+      clear H1 H2.
       invert H; invert H2.
-      + apply le_lt_Sn_m in H7; clear H8 H9.
-        exact (pkplus (Hprev H4 H5 H6) (pkmul H1 (Vector.nth inputs (Fin.of_nat_lt H7)))).
-      + apply le_lt_Sn_m in H8; clear H7 H9.
-        exact (pkplus (Hprev H4 H5 H6) (pkmul H1 (Vector.nth outputs (Fin.of_nat_lt H8)))).
-      + apply le_lt_Sn_m in H9; clear H7 H8.
-        exact (pkplus (Hprev H4 H5 H6) (pkmul H1 (Vector.nth vars (Fin.of_nat_lt H9)))).
-      + exact (pkplus (Hprev H4 H5 H6) H1).
+      + apply le_lt_Sn_m in H5.
+        exact (pkplus (Hprev H3 H4) (pkmul H1 (Vector.nth inputs (Fin.of_nat_lt H5)))).
+      + exact (pkplus (Hprev H3 H4) (pkmul H1 output)).
+      + apply le_lt_Sn_m in H6.
+        exact (pkplus (Hprev H3 H4) (pkmul H1 (Vector.nth vars (Fin.of_nat_lt H6)))).
+      + exact (pkplus (Hprev H3 H4) H1).
   Defined.
 
-  Fixpoint eval_constraint{i o v i' o' v'}
-           (ctr: @constraint i o v)
+  Fixpoint eval_constraint{i v i' v'}
+           (ctr: @constraint i v)
            (inputs: Vfp i')
-           (outputs: Vfp o')
-           (vars: Vfp v') : i <= i' -> o <= o' -> v <= v' -> Fp.
+           (output: Fp)
+           (vars: Vfp v') : i <= i' -> v <= v' -> Fp.
     invert ctr.
     intros.
     pose proof (Nat.max_lub_r _ _ _ H).
@@ -159,24 +155,20 @@ Module R1CS(PF: GaloisField).
     pose proof (Nat.max_lub_l _ _ _ H0).
     pose proof (Nat.max_lub_l _ _ _ H1).
     pose proof (Nat.max_lub_r _ _ _ H2).
-    pose proof (Nat.max_lub_r _ _ _ H3).
-    pose proof (Nat.max_lub_r _ _ _ H4).
     pose proof (Nat.max_lub_l _ _ _ H2).
-    pose proof (Nat.max_lub_l _ _ _ H3).
-    pose proof (Nat.max_lub_l _ _ _ H4).    
-    clear H H0 H1 H2 H3 H4.
-    pose proof (eval_additions A inputs outputs vars H5 H6 H7) as SumA.
-    pose proof (eval_additions B inputs outputs vars H11 H12 H13) as SumB.
-    pose proof (eval_additions C inputs outputs vars H8 H9 H10) as SumC.
+    clear H H0 H1 H2.
+    pose proof (eval_additions A inputs output vars H4 H5) as SumA.
+    pose proof (eval_additions B inputs output vars H6 H8) as SumB.
+    pose proof (eval_additions C inputs output vars H3 H7) as SumC.
     exact (pksub (pkmul SumA SumB) SumC). (** A * B - C *)
   Defined.
 
   Import VectorNotations.
-  Fixpoint eval_fix{n i o v i' o' v'}
-           (r: @r1cs n i o v)
+  Fixpoint eval_fix{n i v i' v'}
+           (r: @r1cs n i v)
            (inputs: Vfp i')
-           (outputs: Vfp o')
-           (vars: Vfp v'): i <= i' -> o <= o' -> v <= v' -> Vfp n.
+           (output: Fp)
+           (vars: Vfp v'): i <= i' -> v <= v' -> Vfp n.
   Proof.
     intros.
     invert r.
@@ -185,31 +177,29 @@ Module R1CS(PF: GaloisField).
       pose proof (Nat.max_lub_l _ _ _ H).
       pose proof (Nat.max_lub_r _ _ _ H0).
       pose proof (Nat.max_lub_l _ _ _ H0).
-      pose proof (Nat.max_lub_r _ _ _ H1).
-      pose proof (Nat.max_lub_l _ _ _ H1).      
-      pose proof (eval_fix _ _ _ _ _ _ _ H3 inputs outputs vars H4 H6 H8) as Hprev.
-      pose proof (eval_constraint H2 inputs outputs vars H5 H7 H9) as CtrEval.
+      pose proof (eval_fix _ _ _ _ _ H2 inputs output vars H3 H5) as Hprev.
+      pose proof (eval_constraint H1 inputs output vars H4 H6) as CtrEval.
       exact (CtrEval :: Hprev). 
   Defined.
 
-  Definition eval{n i o v i' o' v'}
-             (r: @r1cs n i o v)(inputs: Vfp i')(outputs: Vfp o')(vars: Vfp v')
-             {Hi: i <= i'} {Ho: o <= o'} {Hv: v <= v'} :=
-    @eval_fix n i o v i' o' v' r inputs outputs vars Hi Ho Hv.
+  Definition eval{n i v i' v'}
+             (r: @r1cs n i v)(inputs: Vfp i')(output: Fp)(vars: Vfp v')
+             {Hi: i <= i'} {Hv: v <= v'} :=
+    @eval_fix n i v i' v' r inputs output vars Hi Hv.
   
-  Definition correct_lt{n i o v i' o' v'}
-             (r: @r1cs n i o v)(inputs: Vfp i')(outputs: Vfp o')(vars: Vfp v')
-             {Hi: i <= i'}{Ho: o <= o'}{Hv: v <= v'}: Prop :=
-    let values := @eval n i o v i' o' v' r inputs outputs vars Hi Ho Hv in
+  Definition correct_lt{n i v i' v'}
+             (r: @r1cs n i v)(inputs: Vfp i')(output: Fp)(vars: Vfp v')
+             {Hi: i <= i'}{Hv: v <= v'}: Prop :=
+    let values := @eval n i v i' v' r inputs output vars Hi Hv in
     Vector.Forall (fun v => v = 0:%p) values.
 
-  Definition correct{n i o v}(r: @r1cs n i o v)(inputs: Vfp i)(outputs: Vfp o)(vars: Vfp v): Prop :=
-    @correct_lt n i o v i o v r inputs outputs vars (Nat.le_refl i)(Nat.le_refl o)(Nat.le_refl v).
+  Definition correct{n i v}(r: @r1cs n i v)(inputs: Vfp i)(output: Fp)(vars: Vfp v): Prop :=
+    @correct_lt n i v i v r inputs output vars (Nat.le_refl i)(Nat.le_refl v).
 
   Import VectorNotations.
   Unset Printing Implicit.
   Lemma example_correct1:
-    correct <[ { (1i[0]) * (1i[1]) == (1o[0]) } ]> [1:%p; 1:%p] [1:%p] [].
+    correct <[ { (1i[0]) * (1i[1]) == (1o) } ]> [1:%p; 1:%p] (1:%p) [].
   Proof.
     unfold correct, correct_lt.
     cbn.
